Protocol/main.fst
@@ -1,12 +1,14 @@
-#light
 module Main
-open Protocol
-open Client
 
-val main: sp:prin -> res:uri -> user:string -> password:string -> unit
-let main sp resource user password = 
-	print_string "Entering Main";
-	let req = HttpGet resource in
-		let message = client sp req user password in
-		()
-end
+open Protocol
+open Browser
+open Serviceprovider
+open Identityprovider
+
+let main attacker =
+	let sppk, spsk = keygen "https://serviceprovider.org" in 
+	let idppk, idpsk = keygen "https://identityprovider.org" in 
+	fork [	attacker;
+		(fun () -> browser "browser" "https://serviceprovider.org/protectedresource" "me" "myPassword");
+		(fun () -> serviceprovider "https://serviceprovider.org" sppk spsk "browser" "https://identityprovider.org" idppk);
+		(fun () -> identityprovider "https://identityprovider.org" idppk idpsk "browser" "https://serviceprovider.org" sppk)]
